provided decidability instances. provided has_repr instances to display a stream of strings after it has been transformed by a command
'

src/shell_commands.lean
@@ -1,4 +1,5 @@
 import data.list.sort
+import data.string.basic
 import .utils
 
 /-
@@ -35,33 +36,53 @@ structure stream_of_strings :=
   (per_line : list line_pred)
   (bet_line : list doc_pred)
 
+instance : has_repr record := ⟨λ r, utils.list_to_string r⟩
+instance : has_repr stream_of_strings := ⟨λ sos, list.repr sos.records⟩
+
+-- TODO: why can't I use keyword `lemma` here? 
+
 /-                                  -/
 /-               SORT               -/
 /-                                  -/
 
 -- ordering predicates on pairs of records (order ascdending or descending by the first column)
 -- TODO: make more sophisticated (if first col is equal, move to second col and so on)
-def record_asc : record → record → Prop 
-| r1 r2 := (list.head r1) < (list.head r2)
-def record_des : record → record → Prop 
+def record_le : record → record → Prop 
+| r1 r2 := (list.head r1) ≤ (list.head r2)
+def record_gt : record → record → Prop
 | r1 r2 := (list.head r1) > (list.head r2)
 
+instance : has_le record := { le := λ r1 r2, record_le r1 r2, }
+
+instance : decidable_rel record_le :=
+begin
+  rw decidable_rel,
+  intros r1 r2,
+  apply string.decidable_le,
+end
+
+instance : decidable_rel record_gt :=
+begin
+  rw decidable_rel,
+  intros r1 r2,
+  apply string.decidable_lt,
+end
+
 -- sort a list of records ascending
-def sort_asc [h_asc : decidable_rel record_asc] : list record → list record 
-| r := list.merge_sort record_asc r
+def sort_asc (rs : list record) : list record := list.merge_sort record_le rs 
 -- sort a list of records descending
-def sort_des [h_des : decidable_rel record_des] : list record → list record 
-| r := list.merge_sort record_des r
+def sort_des (rs : list record) : list record := list.merge_sort record_gt rs 
+
 
 -- sorted predicates on a list of records
 def sorted_asc : list record → Prop 
-| r := list.sorted record_asc r
+| r := list.sorted record_le r
 def sorted_des : list record → Prop 
-| r := list.sorted record_des r
+| r := list.sorted record_gt r
 
 -- sort
 -- sort in ascending order
-def sort [h_asc : decidable_rel record_asc] : stream_of_strings → stream_of_strings
+def sort : stream_of_strings → stream_of_strings
 | r := { records := sort_asc r.records,
          column_types := r.column_types,
          per_line := r.per_line,
@@ -69,7 +90,7 @@ def sort [h_asc : decidable_rel record_asc] : stream_of_strings → stream_of_st
 
 -- sort -r
 -- sort in descending order
-def sort_r [h_des : decidable_rel record_des] : stream_of_strings → stream_of_strings 
+def sort_r : stream_of_strings → stream_of_strings 
 | r := { records := sort_des r.records,
          column_types := r.column_types,
          per_line := r.per_line,
@@ -77,24 +98,24 @@ def sort_r [h_des : decidable_rel record_des] : stream_of_strings → stream_of_
 
 -- sort -n
 -- sort in ascending order, first column has numeric type
-def sort_n_hlp [h_asc : decidable_rel record_asc] : stream_of_strings → list type → option stream_of_strings 
+def sort_n_hlp : stream_of_strings → list type → option stream_of_strings 
 | sos (type.num :: ts) := some {records := sort_asc sos.records,
                                 column_types := sos.column_types,
                                 per_line := sos.per_line,
                                 bet_line := [sorted_asc]}
 | _ _ := none
-def sort_n [h_asc : decidable_rel record_asc] : stream_of_strings → option stream_of_strings
+def sort_n : stream_of_strings → option stream_of_strings
 | r := sort_n_hlp r r.column_types
 
 -- sort -rn
 -- sort in descending order, first column has numeric type
-def sort_rn_hlp [h_des : decidable_rel record_des] : stream_of_strings → list type → option stream_of_strings 
+def sort_rn_hlp [h_gt : decidable_rel record_gt] : stream_of_strings → list type → option stream_of_strings 
 | sos (type.num :: ts) := some {records := sort_des sos.records,
                                 column_types := sos.column_types,
                                 per_line := sos.per_line,
                                 bet_line := [sorted_des]}
 | _ _ := none
-def sort_rn (input : stream_of_strings) [h_des : decidable_rel record_des]: option stream_of_strings := 
+def sort_rn (input : stream_of_strings) [h_gt : decidable_rel record_gt]: option stream_of_strings := 
   sort_rn_hlp input input.column_types
 
 /-                                  -/
@@ -105,7 +126,7 @@ def sort_rn (input : stream_of_strings) [h_des : decidable_rel record_des]: opti
 def adj_lines_uniq (input : list record) : Prop := sorry
 
 -- collapse adjacent duplicate records
-def make_uniq [h : linear_order record] : list record → list record 
+def make_uniq : list record → list record 
 | (r1 :: (r2 :: rs)) := if r1 = r2 
                         then (r1 :: make_uniq rs) 
                         else (r1 :: (r2 :: make_uniq rs))
@@ -115,17 +136,17 @@ def make_uniq [h : linear_order record] : list record → list record
 def prefix_init_count : list record → list record 
 | (r :: rs) := (((to_string 1) :: r) :: prefix_init_count rs)
 | [] := []
-def make_uniq_c_hlp [h : linear_order record] : list record → list record 
+def make_uniq_c_hlp : list record → list record 
 | ((cnt1 :: rs1) :: ((cnt2 :: rs2) :: rs)) := if rs1 = rs2 
                                               then ((to_string ((utils.string_to_nat cnt1) + (utils.string_to_nat cnt2)) :: rs1) :: make_uniq rs) 
                                               else ((cnt1 :: rs1) :: ((cnt2 :: rs2) :: make_uniq rs))
 | e := e
-def make_uniq_c [h : linear_order record] : list record → list record 
+def make_uniq_c : list record → list record 
 | rs := make_uniq_c_hlp (prefix_init_count rs)
 
 -- uniq
 -- filter out adjacent repeated lines
-def uniq (input : stream_of_strings) [h : linear_order record] : stream_of_strings := 
+def uniq (input : stream_of_strings) : stream_of_strings := 
   { records := make_uniq input.records,
     column_types := input.column_types,
     per_line := input.per_line,
@@ -134,35 +155,63 @@ def uniq (input : stream_of_strings) [h : linear_order record] : stream_of_strin
 -- uniq -c
 -- filter out adjacent repeated lines and prefix the lines with 
 -- a count column
-def uniq_c (input : stream_of_strings) [h : linear_order record] : stream_of_strings := 
+def uniq_c (input : stream_of_strings) : stream_of_strings := 
   { records := make_uniq_c input.records,
     column_types := type.num :: input.column_types,
     per_line := input.per_line,
     bet_line := adj_lines_uniq :: input.bet_line }
 
 /-                                  -/
+/-           DECIDABILITY           -/
+/-                                  -/
+
+-- TODO: need string.le_trans
+def record_linear_order : linear_order record :=
+{ le := record_le,
+  le_refl := begin intro a, simp, rw record_le, simp end,
+  le_trans := begin intros a b c, simp, repeat {rw record_le}, intros hab hbc, sorry end,
+  lt_iff_le_not_le := sorry,
+  le_antisymm := sorry,
+  le_total := sorry,
+  decidable_le := record_le.decidable_rel, }
+
+/-                                  -/
 /-           VERIFICATION           -/
 /-                                  -/
 
--- prove `decidable_rel record_asc` as a separate lemma
--- prove `decidable_rel record_des` as a separate lemma
--- prove `linear_order record` as a separate lemma
-
 def my_sos : stream_of_strings :=
 { records := [["Hello", " ", "world!"],
+              ["Hello", " ", "world!"],
               ["Why,", " ", "hello."],
-              ["Hello", " ", "world!"]],
+              ["Hello", " ", "world!"],
+              ["ABC"],
+              ["ABC"],
+              ["ABC", " "]],
   column_types := [type.str, type.str, type.str],
   per_line := [],
   bet_line := [] }
 
+def my_sos_uniq : stream_of_strings := uniq my_sos
+def my_sos_uniq_c : stream_of_strings := uniq_c my_sos
+def my_sos_sort : stream_of_strings := sort my_sos
+def my_sos_sort_r : stream_of_strings := sort_r my_sos
+
+#eval my_sos_uniq.records
+#eval my_sos_uniq_c.records
+#eval my_sos_sort.records
+#eval my_sos_sort_r.records
+
 -- a composition of sorts flattens to the outermost sort, 
 -- in this case composing sort_r with sort
-lemma sort_composition (sos : stream_of_strings) [h_asc : decidable_rel record_asc] [h_des : decidable_rel record_des] : sort sos = sort (sort_r sos)
-  := sorry
+lemma sort_composition (sos : stream_of_strings) [h_le : decidable_rel record_le] [h_gt : decidable_rel record_gt] : sort sos = sort (sort_r sos) :=
+begin
+  sorry
+end
 
 -- sorting then doing uniq produces a stream of strings without duplicate lines
-lemma sort_then_uniq_nodup (sos : stream_of_strings) [h_asc : decidable_rel record_asc] [h : linear_order record] : list.nodup (uniq (sort sos)).records
-  := sorry
+lemma sort_then_uniq_nodup (sos : stream_of_strings) [h_le : decidable_rel record_le] [h : linear_order record] : list.nodup (uniq (sort sos)).records :=
+begin
+  sorry
+end
 
 end shell
